user 3, session 11481, part 4

diffs-annotated-fixed-2/3/user-3-session-11481.v
@@ -42,6 +42,116 @@ Theorem incX_test :
      recovered := fun _ state' => False |}) incX vars.recover vars.abstr.
 Proof.
 (unfold incX).
-step_proc_basic.
+step_proc.
+(simpl).
+step_proc.
+(simpl).
+step_proc.
+Add Search Blacklist "Raw" "Proofs".
+Set Search Output Name Only.
+Redirect "/var/folders/5x/1mdbpbjd7012l971fq0zkj2w0000gn/T/coqFEFCca"
+SearchPattern _.
+Remove Search Blacklist "Raw" "Proofs".
+Unset Search Output Name Only.
+Qed.
+Theorem incX_ok :
+  proc_spec
+    (fun (_ : unit) state =>
+     {|
+     pre := True;
+     post := fun r state' =>
+             state' =
+             mkState (StateX state + 1) (StateY state) (StateZ state);
+     recovered := fun _ state' => False |}) incX vars.recover vars.abstr.
+Proof.
+(unfold incX).
+(repeat step_proc).
+Add Search Blacklist "Raw" "Proofs".
+Set Search Output Name Only.
+Redirect "/var/folders/5x/1mdbpbjd7012l971fq0zkj2w0000gn/T/coqJPf9xF"
+SearchPattern _.
+Remove Search Blacklist "Raw" "Proofs".
+Unset Search Output Name Only.
+Qed.
+Hint Resolve incX_ok: core.
+Opaque incX.
+Theorem incX_ok_seems_good :
+  proc_spec
+    (fun (_ : unit) state =>
+     {|
+     pre := state = mkState 5 5 5;
+     post := fun r state' => state' = mkState 6 5 5;
+     recovered := fun _ state' => False |}) incX vars.recover vars.abstr.
+Proof.
+(repeat step_proc).
+Add Search Blacklist "Raw" "Proofs".
+Set Search Output Name Only.
+Redirect "/var/folders/5x/1mdbpbjd7012l971fq0zkj2w0000gn/T/coqlGaLOM"
+SearchPattern _.
+Remove Search Blacklist "Raw" "Proofs".
+Unset Search Output Name Only.
+Qed.
+Definition swapXY : proc unit :=
+  x <- vars.read VarX;
+  y <- vars.read VarY; _ <- vars.write VarX y; _ <- vars.write VarY x; Ret tt.
+Redirect "/var/folders/5x/1mdbpbjd7012l971fq0zkj2w0000gn/T/coqEL7D1S"
+Print Ltac Signatures.
+Timeout 1 Print Grammar tactic.
+Add Search Blacklist "Raw" "Proofs".
+Set Search Output Name Only.
+Redirect "/var/folders/5x/1mdbpbjd7012l971fq0zkj2w0000gn/T/coqohJAHb"
+SearchPattern _.
+Remove Search Blacklist "Raw" "Proofs".
+Unset Search Output Name Only.
+Theorem swapXY_ok :
+  proc_spec
+    (fun (_ : unit) state =>
+     {|
+     pre := True;
+     post := fun r state' =>
+             state' = mkState (StateY state) (StateX state) (StateZ state);
+     recovered := fun _ state' => False |}) swapXY vars.recover vars.abstr.
+Proof.
+(repeat step_proc).
+Qed.
+Hint Resolve swapXY_ok: core.
+Opaque swapXY.
+Theorem swapXY_ok_seems_good :
+  proc_spec
+    (fun (_ : unit) state =>
+     {|
+     pre := state = mkState 2 3 4;
+     post := fun r state' => state' = mkState 3 2 4;
+     recovered := fun _ state' => False |}) swapXY vars.recover vars.abstr.
+Proof.
+step_proc.
+Add Search Blacklist "Raw" "Proofs".
+Set Search Output Name Only.
+Redirect "/var/folders/5x/1mdbpbjd7012l971fq0zkj2w0000gn/T/coqYuTOmp"
+SearchPattern _.
+Remove Search Blacklist "Raw" "Proofs".
+Unset Search Output Name Only.
+Qed.
+Definition inc1 (v1 : var) : proc unit :=
+  v <- vars.read v1; _ <- vars.write v1 (1 + v); Ret tt.
+Redirect "/var/folders/5x/1mdbpbjd7012l971fq0zkj2w0000gn/T/coqx7Png1"
+Print Ltac Signatures.
+Timeout 1 Print Grammar tactic.
+Add Search Blacklist "Raw" "Proofs".
+Set Search Output Name Only.
+Redirect "/var/folders/5x/1mdbpbjd7012l971fq0zkj2w0000gn/T/coqSEfhnW"
+SearchPattern _.
+Remove Search Blacklist "Raw" "Proofs".
+Unset Search Output Name Only.
+Definition inc1X_ok :
+  proc_spec
+    (fun (_ : unit) state =>
+     {|
+     pre := True;
+     post := fun r state' =>
+             state' =
+             mkState (1 + StateX state) (StateY state) (StateZ state);
+     recovered := fun _ state' => True |}) (inc1 VarX) vars.recover
+    vars.abstr.
 (* Auto-generated comment: Succeeded. *)
 
